pcuic/theories/PCUICCumulativity.v
@@ -1,0 +1,108 @@
+(* Distributed under the terms of the MIT license.   *)
+From Equations Require Import Equations.
+From Coq Require Import Bool String List Program BinPos Compare_dec Omega.
+From Template Require Import config utils univ.
+From PCUIC Require Import PCUICAst PCUICAstUtils PCUICInduction
+     PCUICLiftSubst PCUICUnivSubst PCUICTyping PCUICWeakeningEnv PCUICWeakening
+     PCUICSubstitution PCUICClosed.
+Require Import ssreflect ssrbool.
+Require Import String.
+Require Import LibHypsNaming.
+Local Open Scope string_scope.
+Set Asymmetric Patterns.
+
+Existing Instance config.default_checker_flags.
+
+Reserved Notation " Σ ;;; Γ |- t == u " (at level 50, Γ, t, u at next level).
+
+Lemma red_step Σ Γ t u v : red1 Σ Γ t u -> red Σ Γ u v -> red Σ Γ t v.
+Proof.
+  induction 2. econstructor; auto. constructor. apply X.
+  econstructor 2; eauto.
+Qed.
+
+Require Import Equations.Type.Relation Equations.Type.Relation_Properties.
+
+Lemma red_alt@{i j +} Σ Γ t u : red Σ Γ t u <~> clos_refl_trans@{i j} (red1 Σ Γ) t u.
+Proof.
+  split. intros H. apply clos_rt_rtn1_iff.
+  induction H; econstructor; eauto.
+  intros H. apply clos_rt_rtn1_iff in H.
+  induction H; econstructor; eauto.
+Qed.
+
+Lemma cumul_alt Σ Γ t u :
+  Σ ;;; Γ |- t <= u <~> { v & { v' & (red Σ Γ t v * red Σ Γ u v' * leq_term (snd Σ) v v')%type } }.
+Proof.
+  split.
+  { induction 1. exists t, u. intuition auto; constructor.
+    destruct IHX as (v' & v'' & (redv & redv') & leqv).
+    exists v', v''. intuition auto. now eapply red_step.
+    destruct IHX as (v' & v'' & (redv & redv') & leqv).
+    exists v', v''. intuition auto. now eapply red_step. }
+  { intros [v [v' [[redv redv'] Hleq]]]. apply red_alt in redv. apply red_alt in redv'.
+    apply clos_rt_rt1n in redv.
+    apply clos_rt_rt1n in redv'.
+    induction redv. induction redv'. constructor; auto.
+    econstructor 3; eauto.
+    econstructor 2; eauto. }
+Qed.
+
+Inductive conv_alt `{checker_flags} (Σ : global_context) (Γ : context) : term -> term -> Type :=
+| conv_alt_refl t u : eq_term (snd Σ) t u = true -> Σ ;;; Γ |- t == u
+| conv_alt_red_l t u v : red1 (fst Σ) Γ t v -> Σ ;;; Γ |- v == u -> Σ ;;; Γ |- t == u
+| conv_alt_red_r t u v : Σ ;;; Γ |- t == v -> red1 (fst Σ) Γ u v -> Σ ;;; Γ |- t == u
+where " Σ ;;; Γ |- t == u " := (@conv_alt _ Σ Γ t u) : type_scope.
+
+Lemma red_conv_alt Σ Γ t u : red (fst Σ) Γ t u -> Σ ;;; Γ |- t == u.
+Proof.
+  intros. apply red_alt in X. apply clos_rt_rt1n_iff in X.
+  induction X. constructor. apply eq_term_refl.
+  apply clos_rt_rt1n_iff in X. apply red_alt in X.
+  econstructor 2; eauto.
+Qed.
+Hint Resolve red_conv_alt.
+
+Lemma red1_red (Σ : global_context) Γ t u : red1 (fst Σ) Γ t u -> red (fst Σ) Γ t u.
+Proof. econstructor; eauto. constructor. Qed.
+Hint Resolve red1_red.
+
+Lemma leq_term_antisym Σ t u : leq_term Σ t u -> leq_term Σ u t -> eq_term Σ t u.
+Proof.
+Admitted.
+
+Lemma leq_term_refl Σ t : leq_term Σ t t.
+Proof. apply eq_term_leq_term, eq_term_refl. Qed.
+
+Lemma eq_term_sym Σ t u : eq_term Σ t u -> eq_term Σ u t.
+Proof.
+Admitted.
+
+Lemma cumul_refl' Σ Γ t : cumul Σ Γ t t.
+Proof. apply cumul_refl, leq_term_refl. Qed.
+
+Hint Resolve leq_term_refl cumul_refl' : core.
+
+Lemma cumul_conv_alt Σ Γ t u :
+  Σ ;;; Γ |- t <= u -> Σ ;;; Γ |- u <= t -> Σ ;;; Γ |- t == u.
+             (* (forall v, Σ ;;; Γ |- u == v -> Σ ;;; Γ |- t == v). *)
+Proof.
+  intros H. apply cumul_alt in H.
+  destruct H as (v & v' & (redv & redv') & leqv).
+  intros H'. apply cumul_alt in H'.
+  destruct H' as (v0 & v'0 & (redv0 & redv'0) & leqv0).
+  (** Needs confluence to show the two redexes can be joined *)
+Admitted.
+
+
+
+Lemma conv_conv_alt Σ Γ t u : Σ ;;; Γ |- t = u <~> Σ ;;; Γ |- t == u.
+Proof.
+  split; induction 1. apply cumul_conv_alt in b; auto.
+  constructor; constructor. now eapply eq_term_leq_term.
+  eapply eq_term_leq_term; now apply eq_term_sym.
+  constructor. econstructor 2; eauto. apply IHX.
+  econstructor 3. 2:eauto. apply IHX.
+  constructor. econstructor 3. 2:eauto. apply IHX.
+  econstructor 2; eauto. apply IHX.
+Qed.
